lib/hst/Hacl.Cast.fst
@@ -30,10 +30,10 @@ assume val uint64_to_sint8: a:UInt64.t -> Tot (b:S8.t{S8.v b = UInt64.v a % pow2
 
 assume val uint32_to_sint128: a:UInt32.t -> Tot (b:S128.t{S128.v b = UInt32.v a})
 assume val uint32_to_sint64: a:UInt32.t -> Tot (b:S64.t{S64.v b = UInt32.v a})
-assume val uint32_to_sint32: a:UInt32.t -> Tot (b:S32.t{S32.v b = UInt32.v a % pow2 32})
+assume val uint32_to_sint32: a:UInt32.t -> Tot (b:S32.t{S32.v b = UInt32.v a})
 assume val uint32_to_sint8: a:UInt32.t -> Tot (b:S8.t{S8.v b = UInt32.v a % pow2 8})
 
 assume val uint8_to_sint128: a:UInt8.t -> Tot (b:S128.t{S128.v b = UInt8.v a})
 assume val uint8_to_sint64: a:UInt8.t -> Tot (b:S64.t{S64.v b = UInt8.v a})
-assume val uint8_to_sint32: a:UInt8.t -> Tot (b:S32.t{S32.v b = UInt8.v a % pow2 32})
-assume val uint8_to_sint8: a:UInt8.t -> Tot (b:S8.t{S8.v b = UInt8.v a % pow2 8})
+assume val uint8_to_sint32: a:UInt8.t -> Tot (b:S32.t{S32.v b = UInt8.v a})
+assume val uint8_to_sint8: a:UInt8.t -> Tot (b:S8.t{S8.v b = UInt8.v a})
